\section{Derivation} \label{sec:derivation}

{\tiny
\begin{align*}
C(l_1, l_2, \ldots, 1, \ldots, l_n)
&<
C(l_1, l_2, \ldots, 0, \ldots, l_n) \\
\alpha
+
\alpha \sum_{i \not{=} k} l_i
+
\Big[1 - \frac{1}{n}\Big(1 + \sum_{j\not{=}k} l_j\Big)\Big]^2
+
\sum_{i\not{=}k} \Big[l_i - \frac{1}{n}\Big(1 +  \sum_{j\not{=}k} l_j\Big)\Big]^2
&<
0
+
\alpha \sum_{i \not{=} k} l_i
+
\Big[0 - \Big(\frac{1}{n} \sum_{j\not{=}k} l_j\Big)\Big]^2
+
\sum_{i\not{=}k} \Big[l_i - \frac{1}{n}\Big(0 + \sum_{j\not{=}k} l_j\Big)\Big]^2 \\
\alpha
+
\Big[\Big(1 - \frac{1}{n}\Big) + \frac{1}{n} \sum_{j\not{=}k} l_j\Big]^2
+
\sum_{i\not{=}k} \Big[l_i - \frac{1}{n}\Big(1 +  \sum_{j\not{=}k} l_j\Big)\Big]^2
&<
\Big[ - \Big(\frac{1}{n} \sum_{j\not{=}k} l_j\Big)\Big]^2
+
\sum_{i\not{=}k} \Big[l_i - \frac{1}{n}\Big(\sum_{j\not{=}k} l_j\Big)\Big]^2 \\
\alpha
+
\Big[\Big(1 - \frac{1}{n}\Big) + \frac{1}{n} \sum_{j\not{=}k} l_j\Big]^2
+
\sum_{i\not{=}k} \Big[l_i^2 - \frac{2l_i}{n}\Big(1 +  \sum_{j\not{=}k} l_j\Big) + \Big(\frac{1}{n} +  \frac{1}{n}\sum_{j\not{=}k} l_j\Big)^2 \Big]
&<
\Big[\frac{1}{n} \sum_{j\not{=}k} l_j\Big]^2
+
\sum_{i\not{=}k}
\Big[
l_i^2 - \frac{2l_i}{n}\Big(\sum_{j\not{=}k} l_j\Big) + \Big(\frac{1}{n}\sum_{j\not{=}k} l_j\Big)^2
\Big]\\
\alpha
+
\Big[\Big(1 - \frac{1}{n}\Big) + \frac{1}{n} \sum_{j\not{=}k} l_j\Big]^2
+
\sum_{i\not{=}k} \Big[ - \frac{2l_i}{n} + \Big(\frac{1}{n} +  \frac{1}{n}\sum_{j\not{=}k} l_j\Big)^2 \Big]
&<
\Big[\frac{1}{n} \sum_{j\not{=}k} l_j\Big]^2
+
\sum_{i\not{=}k}
\Big(\frac{1}{n}\sum_{j\not{=}k} l_j\Big)^2
\\
\alpha
+
\Big[\Big(1 - \frac{1}{n}\Big) + \frac{1}{n} \sum_{j\not{=}k} l_j\Big]^2
+
\sum_{i\not{=}k} \Big[ - \frac{2l_i}{n} + \frac{1}{n^2} +  \frac{2}{n^2}\sum_{j\not{=}k} l_j  + \Big(\frac{1}{n}\sum_{j\not{=}k} l_j\Big)^2 \Big]
&<
\Big[\frac{1}{n} \sum_{j\not{=}k} l_j\Big]^2
+
\sum_{i\not{=}k}
\Big(\frac{1}{n}\sum_{j\not{=}k} l_j\Big)^2
\\
\alpha
+
\Big[\Big(1 - \frac{1}{n}\Big) + \frac{1}{n} \sum_{j\not{=}k} l_j\Big]^2
+
\sum_{i\not{=}k} \Big[ - \frac{2l_i}{n} + \frac{1}{n^2} +  \frac{2}{n^2}\sum_{j\not{=}k} l_j  \Big]
&<
\Big[\frac{1}{n} \sum_{j\not{=}k} l_j\Big]^2
\\
\alpha
+
\Big(1 - \frac{1}{n}\Big)^2 + \Big(1 - \frac{1}{n}\Big)\frac{2}{n} \sum_{j\not{=}k} l_j + \Big[\frac{1}{n} \sum_{j\not{=}k} l_j\Big]^2
+
\sum_{i\not{=}k} \Big[ - \frac{2l_i}{n} + \frac{1}{n^2} +  \frac{2}{n^2}\sum_{j\not{=}k} l_j  \Big]
&<
\Big[\frac{1}{n} \sum_{j\not{=}k} l_j\Big]^2
\\
\alpha
+
\Big(1 - \frac{1}{n}\Big)^2 + \Big(1 - \frac{1}{n}\Big)\frac{2}{n} \sum_{j\not{=}k} l_j
+
\sum_{i\not{=}k} \Big[ - \frac{2l_i}{n} + \frac{1}{n^2} +  \frac{2}{n^2}\sum_{j\not{=}k} l_j  \Big]
&<
0
\\
\alpha
+
\Big(1 - \frac{1}{n}\Big)^2 + \Big(1 - \frac{1}{n}\Big)\frac{2}{n} \sum_{j\not{=}k} l_j
-
\frac{2}{n} \sum_{i\not{=}k} \Big[ l_i \Big]
+ \frac{n-1}{n^2} +  \frac{2(n-1)}{n^2}\sum_{j\not{=}k} l_j
&<
0
\\
\alpha
+
\Big(1 - \frac{1}{n}\Big)^2 + \Big(\frac{2}{n} - \frac{2}{n^2}\Big) \sum_{j\not{=}k} l_j
-
\frac{2}{n} \sum_{i\not{=}k} \Big[ l_i \Big]
+ \frac{n-1}{n^2}
+  \Big(\frac{2}{n} + \frac{-2}{n^2} \Big)
\sum_{j\not{=}k} l_j
&<
0
\\
\alpha
+
\Big(1 - \frac{1}{n}\Big)^2 + \Big(\frac{2}{n} - \frac{2}{n^2}\Big) \sum_{j\not{=}k} l_j
+ \frac{n-1}{n^2}
+ \frac{-2}{n^2}
\sum_{j\not{=}k} l_j
&<
0
\\
\alpha
+
1 - \frac{2}{n} + \frac{1}{n^2}
+ \frac{1}{n}
+ \frac{-1}{n^2}
+
\Big(
\frac{-4}{n^2}
+
\frac{2}{n}
\Big)
\sum_{j\not{=}k} l_j
&<
0
\\
\alpha
+
1
- \frac{1}{n}
+
\Big(
\frac{-4}{n^2}
+
\frac{2}{n}
\Big)
\sum_{j\not{=}k} l_j
&<
0
\\
\end{align*}
}
